HC/ZK.ec
@@ -11,30 +11,49 @@ import OMZK.
 clone import StatisticalZKDeriv with op negl <- 2%r * negl + 20%r * negl2.
 axiom negl2_prop : 0%r <= negl2 < 1%r/4%r.
 
-lemma sim1_rew_ph :         forall (V <: MaliciousVerifier) , forall (x : (glob V) * (glob Sim1)),
-  phoare[ Sim1(V).run :
-           ((glob V), (glob Sim1)) = x ==> ((glob V), (glob Sim1)) = x] = 1%r.
-admitted.
+require RewBasics.
+clone import RewBasics as Rew with type sbits <- sbits.
 
-lemma hc_statistical_zk:
-        forall (V <: MaliciousVerifier{HonestProver, OMZK.MW.IFB.IM.W, OMZK.MW.IFB.DW}) 
-               (D <: ZKDistinguisher{HonestProver, OMZK.MW.IFB.IM.W, V}),
-        (forall (V0 <: MaliciousVerifier), islossless V0.challenge => islossless V0.summitup => islossless Sim1(V0).run) =>
-        forall stat wit ax N &m,
-        islossless V.summitup => islossless V.challenge => islossless D.guess =>
-        forall (V0 <: MaliciousVerifier), 
+section.
+
+declare module V : MaliciousVerifier{HonestProver, OMZK.MW.IFB.IM.W, OMZK.MW.IFB.DW}.
+declare module D : ZKDistinguisher{HonestProver, OMZK.MW.IFB.IM.W, V}.
+
+
+axiom Sim1_run_ll : forall (V0 <: MaliciousVerifier), islossless V0.challenge => islossless V0.summitup => islossless Sim1(V0).run.
+
+axiom V_summitup_ll : islossless V.summitup. 
+axiom V_challenge_ll : islossless V.challenge.
+axiom D_guess_ll : islossless D.guess.
+
+
+axiom rewindable_V_plus : 
+        (exists (f : glob V -> sbits),
+         injective f /\
+         (forall &m, Pr[ V.getState() @ &m : (glob V) = ((glob V){m})
+                                          /\ res = f ((glob V){m} ) ] = 1%r) /\
+         (forall &m b (x: glob V), b = f x =>
+           Pr[V.setState(b) @ &m : glob V = x] = 1%r) /\
+         islossless V.setState).
+
+
+
+lemma hc_statistical_zk stat wit ax N &m:
         IsHC (stat, wit) => 
         0 <= N =>
         let real_prob = Pr[ZKReal(HonestProver, V, D).run(stat, wit, ax) @ &m : res] in
         let ideal_prob = Pr[ZKIdeal(Simulator(Sim1), V, D).run(stat, wit, N, ax) @ &m : res] in
-          `|real_prob - ideal_prob| <= (2%r * negl + 20%r * negl2) + 2%r * (1%r- (1%r/2%r - negl2) ) ^ N.
+          `|real_prob - ideal_prob| <= (2%r * negl + 20%r * negl2) + 2%r * (1%r- (1%r/2%r - negl2)) ^ N.
+proof.
 progress.
-print statistical_zk.
-apply (statistical_zk HonestProver Sim1  V D _ _  _ _ _ _ stat wit ax N
-  (inv 2%r - negl2) &m).
-apply H. auto. auto. auto. apply (sim1_rew_ph V). 
-progress. 
-apply (sim1_prop V0 D0 _ _  _ &m0 p w aux _ ).
-auto. auto. apply negl2_prop.  auto. auto. auto. auto. auto.  auto. 
-apply (sim1assc V D);auto. apply negl2_prop. smt.
+apply (statistical_zk HonestProver Sim1  V D _ _ _ _ _ _ _ stat wit ax N
+  (inv 2%r - negl2) &m). apply Sim1_run_ll. apply V_summitup_ll. apply V_challenge_ll. apply D_guess_ll.
+apply rewindable_V_plus.
+apply (sim1_rew_ph V ). apply V_summitup_ll. apply V_challenge_ll. 
+apply (rewindable_A_plus V). apply rewindable_V_plus.
+progress.
+apply (sim1_prop V D _ _  _ _ _ &m0 p w aux _ ).  apply (rewindable_A_plus V). exists f. split. auto. auto.
+auto. auto.   auto. apply negl2_prop.  auto. auto. auto. 
+apply (sim1assc V D);auto. apply (rewindable_A_plus V). apply rewindable_V_plus. apply D_guess_ll. apply V_summitup_ll.
+apply V_challenge_ll. apply negl2_prop. smt.
 qed.
